@prefix asn: <http://purl.org/asn/schema/core/> .
@prefix cc: "http://creativecommons.org/ns#".
@prefix ceasn: <http://purl.org/ctdlasn/terms/> .
@prefix ceterms: <http://purl.org/ctdl/terms/> .
@prefix dct: <http://purl.org/dc/terms/> .
@prefix owl: <http://www.w3.org/2002/07/owl#> .
@prefix rdf: <http://www.w3.org/1999/02/22-rdf-syntax-ns#> .
@prefix rdfs: <http://www.w3.org/2000/01/rdf-schema#> .
@prefix schema: <http://schema.org/> .
@prefix skos: <http://www.w3.org/2004/02/skos/core#> .
@prefix t3nt: <https://t3innovationnetwork.org/networktrust/terms/>.
@prefix xsd: <http://www.w3.org/2001/XMLSchema#> .

t3nt:Directory a rdfs:Class ;
    rdfs:label "Competency Framework Directory"@en-US .
    dct:identifier "t3nt:Directory" ;
    rdfs:comment "A structured table of contents of the competency framework holdings of a Trust Member registry."@en-US ;
    rdfs:isDefinedBy <https://t3innovationnetwork.org/networktrust/terms/> .

t3nt:FrameworkPackage a rdfs:Class ;
    rdfs:label "Framework Package"@en-US ;
    dct:identifier "t3nt:FrameworkPackage" ;
    rdfs:comment "Container for a requested a competency framework and associated metadata including the URI of the provider registry, transaction date/time stamp and URIs identifying controling use and retention policies for the transmitted competency framework."@en-US ;
    rdfs:isDefinedBy <https://t3innovationnetwork.org/networktrust/terms/> .
    
t3nt:MemberPolicy a rdfs:Class ;
    rdfs:label "Member Policy"@en-US ;
    dct:identifier "t3nt:MemberPolicy" ;
    rdfs:comment "License defining a Trust Member's required permissions and prohibitions regarding the use and retention of one of its competency frameworks by another Trust Member or an end user."@en-US ;
    skos:note "A competency framework always has two distinct member policies, one constraining the behavior of an end user (beneficiary rights) and another constraining the sharing of a competency framework by one Trust Member with another Trust Member (registry rights)."@en-US ;
    rdfs:isDefinedBy <https://t3innovationnetwork.org/networktrust/terms/> .

t3nt:NetworkNodeProvider a rdfs:Class ;
    rdfs:label "Network Node Provider"@en-US ;
    dct:identifier "t3nt:NetworkNodeProvider" ;
    rdfs:comment "Competency framework registry that is a network node provider in good standing."@en-US ;
    rdfs:isDefinedBy <https://t3innovationnetwork.org/networktrust/terms/> .

t3nt:TransactionLog a rdfs:Class ;
    rdfs:label "Transaction Log"@en-US ;
    dct:identifier "t3nt:TransactionLog" ;
    rdfs:comment "An immutable, searchable log of each Trust Network transaction transmitting a Framework Package from one Trust Member to another Trust Member."@en-US ;
    rdfs:isDefinedBy <https://t3innovationnetwork.org/networktrust/terms/> .
    
cc:attributionName a rdfs:Property ;
    rdfs:label "Attribution Name"@en-US ;
    dct:identifier "cc:attributionName" ;
    rdfs:comment "Name of an organization or person to which credit is owed as copyright holder and/or author." ;
    rdfs:domain t3nt:FrameworkPackage, t3nt:TransactionLog ;
    rdfs:range t3nt:MemberPolicy .
    
cc:attributionURL a rdfs:Property ;
    rdfs:label "Attribution Name"@en-US ;
    dct:identifier "cc:attributionName" ;
    rdfs:comment "URL identifying an organization or person to which credit is owed as copyright holder and/or author."
    rdfs:domain t3nt:FrameworkPackage, t3nt:TransactionLog ;
    rdfs:range t3nt:MemberPolicy .

t3nt:beneficiaryRights a rdfs:Property ;
    rdfs:label "End User License"@en-US ;
    dct:identifier "t3nt:beneficiaryRights" ;
    rdfs:comment "Resource defining the permissions and prohibitions on end users of a Trust Member's competency frameworks." ;
    rdfs:domain t3nt:FrameworkPackage, t3nt:TransactionLog ;
    rdfs:range t3nt:MemberPolicy .

t3nt:conditionsOfAccess a rdfs:Property ;
    rdfs:label "Conditions of Access"@en-US ;
    dct:identifier "t3nt:conditionsOfAccess" ;
    rdfs:comment "Statement of constraints on a person or application accessing the resource." ;
    rdfs:domain t3nt:Directory ;
    rdfs:range rdf:langString .

dct:created a rdfs:Property ;
    rdfs:label "Date Created"@en-US ;
    dct:identifier "dct:created" ;
    rdfs:comment "Date of creation of the resource." ;
    rdfs:domain skos:ConceptScheme ;
    rdfs:range xsd:date .
    
dct:creator a rdfs:Property ;
    rdfs:label "Creator"@en-US ;
    dct:identifier "dct:creator" ;
    rdfs:comment "An entity responsible for making the resource." ;
    rdfs:domain skos:ConceptScheme ;
    rdfs:range rdf:langString .

skos:definition a rdfs:Property ;
    rdfs:label "Definition"@en-US ;
    dct:identifier "skos:definition" ;
    rdfs:comment "Statement of the exact meaning of a concept." ;
    rdfs:domain skos:ConceptScheme ;
    rdfs:range rdf:langString .
    
skos:description a rdfs:Property ;
    rdfs:label "Description"@en-US ;
    dct:identifier "skos:definition" ;
    rdfs:comment "An account of the resource." ;
    rdfs:domain skos:ConceptScheme ;
    rdfs:range rdf:langString .
    
t3nt:frameworkLocation a rdfs:Property ;
    rdfs:label "Framework Location"@en-US ;
    dct:identifier "t3nt:frameworklocation" ;
    rdfs:comment "A URI identifying a competency framework in the Directory table of contents." ;
    rdfs:domain t3nt:Directory ;
    rdfs:range ceasn:CommpetencyFramework .

t3nt:frameworkProvider a rdfs:Property ;
    rdfs:label "Framework Provider"@en-US ;
    dct:identifier "t3nt:frameworkProvider" ;
    rdfs:comment "Trust Member registry transmitting a competency framework to a Trust Member registry requesting the framework." ;
    rdfs:domain t3nt:TransactionLog, t3nt:FrameworkPackage ;
    rdfs:range t3nt:NetworkNodeProvider .
    
t3nt:frameworkRequester a rdfs:Property ;
    rdfs:label "Framework Requester"@en-US ;
    dct:identifier "t3nt:frameworkRequester" ;
    rdfs:comment "Trust Member registry requesting transmission of a competency framework from another Trust Member registry." ;
    rdfs:domain t3nt:TransactionLog, t3nt:FrameworkPackage ;
    rdfs:range t3nt:NetworkNodeProvider .

skos:hasTopConcept a rdfs:Property ;
    rdfs:label "Has Top Concept"@en-US ;
    dct:identifier "skos:hasTopConcept" ;
    rdfs:comment "Top concept in a hierarchy of narrower concepts." ;
    rdfs:domain skos:ConceptScheme ;
    rdfs:range skos:Concept .
    
dct:hasPart a rdfs:Property ;
    rdfs:label "Has Part"@en-US ;
    dct:identifier "dct:hasPart" ;
    rdfs:comment "A related resource that is included either physically or logically in the described resource." ;
    rdfs:domain t3nt:Directory ;
    rdfs:range t3nt:DirectoryEntry .
    
dct:isPartOf a rdfs:Property ;
    rdfs:label "Is Part Of"@en-US ;
    dct:identifier "dct:isPartOf" ;
    rdfs:comment "A related resource in which the described resource is physically or logically included." ;
    rdfs:domain t3nt:DirectoryEntry ;
    rdfs:range t3nt:Directory .

skos:inScheme a rdfs:Property ;
    rdfs:label "In Scheme"@en-US ;
    dct:identifier "skos:inScheme" ;
    rdfs:comment "Concept Scheme to which a Concept belongs." ;
    rdfs:domain skos:ConceptScheme ;
    rdfs:range skos:Concept .
    
t3nt:metamodel a rdfs:Property ;
    rdfs:label "Meta-Model"@en-US ;
    dct:identifier "t3nt:metamodel" ;
    rdfs:comment "The competency framework metamodel used for this competency framework model; e.g., ASN, IMS CASE v. 1.0. " ;
    rdfs:domain t3nt:Directory ;
    rdfs:range xsd:anyURI ;
    skos:note "Provide as value the URI of the competency framework metamodel as expressed in the concept scheme CFModels.jsonld."@en-US .

dct:modified a rdfs:Property ;
    rdfs:label "Date Modified"@en-US ;
    dct:identifier "dct:modified" ;
    rdfs:comment "Date on which the resource was changed." ;
    rdfs:domain skos:ConceptScheme ;
    rdfs:range xsd:date .
    
skos:prefLabel a rdfs:Property ;
    rdfs:label "Preferred Label"@en-US ;
    dct:identifier "skos:prefLabel" ;
    rdfs:comment "favored label for a concept among alternatives." ;
    rdfs:domain skos:Concept ;
    rdfs:range rdf:langString .

t3nt:publicationStatus a rdfs:Property ;
    rdfs:label "Publication Status"@en-US ;
    dct:identifier "t3nt:publicationStatus" ;
    rdfs:comment "Reqource identifying the publication status of the entity." ;
    rdfs:domain skos:Concept ;
    rdfs:range skos:Concept .
    
t3nt:registeryRights a rdfs:Property ;
    rdfs:label "Registry Rights"@en-US ;
    dct:identifier "t3nt:registryRights" ;
    rdfs:comment "Resource defining the permissions and prohibitions on a Trust Member's use and retention of another Trust Member's competency framework." ;
    rdfs:domain t3nt:FrameworkPackage, t3nt:TransactionLog ;
    rdfs:range t3nt:MemberPolicy .
    
dct:title a rdfs:Property ;
    rdfs:label "Title"@en-US ;
    dct:identifier "dct:title" ;
    rdfs:comment "Name given to the resource." ;
    rdfs:domain skos:Concept, t3nt:transactionLog ;
    rdfs:range rdf:langString .
    
t3nt:transactionDate" a rdfs:Property ;
    rdfs:label "Transaction Date"@en-US ;
    dct:identifier "t3nt:transactionDate" ;
    rdfs:comment "Date/time of a transaction between two Trust Members transferring a competency framework." ;
    rdfs:domain t3nt:transactionLog ;
    rdfs:range xsd:dateTime .
